Test/git-issues/git-issue-1604c.dfy
@@ -1,12 +1,25 @@
-// RUN: %dafny /compile:3 /rprint:"%t.rprint" /compileTarget:js "%s" > "%t"
-// RUN: %dafny /compile:3 /rprint:"%t.rprint" /compileTarget:java "%s" >> "%t"
-// RUN: %dafny /compile:3 /rprint:"%t.rprint" /compileTarget:go "%s" >> "%t"
-// RUN: %dafny /compile:3 /rprint:"%t.rprint" /compileTarget:cs "%s" >> "%t"
+// RUN: %dafny /compile:0 /rprint:"%t.rprint" /compileTarget:js "%s" > "%t"
+// RUN: %dafny /noVerify /compile:4 /compileTarget:js "%s" > "%t"
+// RUN: %dafny /noVerify /compile:4 /compileTarget:java "%s" >> "%t"
+// RUN: %dafny /noVerify /compile:4 /compileTarget:go "%s" >> "%t"
+// RUN: %dafny /noVerify /compile:4 /compileTarget:cs "%s" >> "%t"
 // RUN: %diff "%s.expect" "%t"
 
 trait Tr { }
 class A extends Tr { }
 class B extends Tr { }
+
+predicate SpecialA(a: A)
+{
+  false
+}
+type Ap  = x : A | SpecialA(x) witness *
+
+function method testSpecial(x: Tr): bool
+  requires x is A && SpecialA(x)
+{
+  1/0 == 0
+}
 
 function method test(x: Tr): bool
   requires x is A
@@ -18,7 +31,12 @@ method Main() {
   var a := new A;
   var b := new B;
   var s: set<Tr> := {a, b};
+  var s2: set<Ap> := {};
   var aa := forall a': A :: a' in s ==> test(a');
-  assert(aa);
+
+  // Fine because Ap has the same type as elements of s2
+  var ab := forall a': Ap | a' in s2 :: testSpecial(a');
+  assert aa;
+  assert ab;
   print "ok";
 }
